***NO_CI*** ulib verifies

ulib/FStar.Buffer.fst
@@ -30,6 +30,7 @@ type buffer (a:Type) = _buffer a
 
 (* Ghost getters for specifications *)
 let contains #a h (b:buffer a) : GTot Type0 = HS.contains h b.content
+let does_not_contain #a h (b:buffer a) : GTot Type0 = HS.does_not_contain h b.content
 
 //17-01-04 notations: 
 //17-01-04 when to use sel, index, get, read? 
@@ -53,10 +54,11 @@ let frameOf #a (b:buffer a) : GTot HH.rid = frameOf (content b)
 
 (* Liveliness condition, necessary for any computation on the buffer *)
 let live #a (h:mem) (b:buffer a) : GTot Type0 = contains h b
+let not_live #a (h:mem) (b:buffer a) : GTot Type0 = does_not_contain h b
 //17-01-04 global pick between live and contains?
 
 val recall: #a:Type
-  -> b:buffer a{is_eternal_region (frameOf b) && not (b.content.mm)} -> Stack unit
+  -> b:buffer a{is_eternal_region (frameOf b) && not (is_mm b.content)} -> Stack unit
   (requires (fun m -> True))
   (ensures  (fun m0 _ m1 -> m0==m1 /\ live m1 b))
 let recall #a b = recall b.content
@@ -82,8 +84,8 @@ let includes #a (x:buffer a) (y:buffer a) : GTot Type0 =
 
 (* Disjointness between two buffers *)
 let disjoint #a #a' (x:buffer a) (y:buffer a') : GTot Type0 =
-  frameOf x <> frameOf y \/ as_aref x =!= as_aref y
-  \/ (a == a' /\ as_aref x == as_aref y /\ frameOf x = frameOf y /\
+  frameOf x <> frameOf y \/ as_addr x <> as_addr y
+  \/ (a == a' /\ as_addr x == as_addr y /\ frameOf x = frameOf y /\ x.max_length = y.max_length /\
      (idx x + length x <= idx y \/ idx y + length y <= idx x))
 
 (* Disjointness is symmetric *)
@@ -106,7 +108,7 @@ let lemma_disjoint_sub' #a #a' (x:buffer a) (subx:buffer a) (y:buffer a') : Lemm
   = ()
 
 val lemma_live_disjoint: #a:Type -> #a':Type -> h:mem -> b:buffer a -> b':buffer a' -> Lemma
-  (requires (live h b /\ ~(contains h b')))
+  (requires (live h b /\ does_not_contain h b'))
   (ensures (disjoint b b'))
   [SMTPatT (disjoint b b'); SMTPatT (live h b)]
 let lemma_live_disjoint #a #a' h b b' = ()
@@ -137,7 +139,7 @@ let lemma_arefs_1 s = Set.lemma_equal_intro (arefs s) (Set.empty)
 
 val lemma_arefs_2: s1:TSet.set abuffer -> s2:TSet.set abuffer -> Lemma
   (requires True)
-  (ensures  (arefs (s1 ++ s2) == arefs s1 ++ arefs s2))
+  (ensures  (arefs (s1 ++ s2) == Set.union (arefs s1) (arefs s2)))
   [SMTPatOr [
     [SMTPat (arefs (s2 ++ s1))];
     [SMTPat (arefs (s1 ++ s2))]
@@ -205,18 +207,25 @@ let modifies_buf_0 rid h h' =
   /\ (forall (#tt:Type) (bb:buffer tt). (frameOf bb = rid /\ live h bb) ==> equal h bb h' bb)
 
 let modifies_buf_1 (#t:Type) rid (b:buffer t) h h' = //would be good to drop the rid argument on these, since they can be computed from the buffers
-  modifies_ref rid !{as_ref b} h h'
+  modifies_ref rid (Set.singleton (Heap.addr_of (as_ref b))) h h'
   /\ (forall (#tt:Type) (bb:buffer tt). (frameOf bb = rid /\ live h bb /\ disjoint b bb) ==> equal h bb h' bb)
+
+let to_set_2 (n1:nat) (n2:nat) :Set.set nat = Set.union (Set.singleton n1) (Set.singleton n2)
 
 let modifies_buf_2 (#t:Type) (#t':Type) rid (b:buffer t) (b':buffer t') h h' =
   modifies_ref rid (to_set_2 (as_addr b) (as_addr b')) h h'
   /\ (forall (#tt:Type) (bb:buffer tt). (frameOf bb = rid /\ live h bb /\ disjoint b bb /\ disjoint b' bb)
        ==> equal h bb h' bb)
 
+let to_set_3 (n1:nat) (n2:nat) (n3:nat) :Set.set nat = Set.union (Set.union (Set.singleton n1) (Set.singleton n2)) (Set.singleton n3)
+
 let modifies_buf_3 (#t:Type) (#t':Type) (#t'':Type) rid (b:buffer t) (b':buffer t') (b'':buffer t'') h h' =
   modifies_ref rid (to_set_3 (as_addr b) (as_addr b') (as_addr b'')) h h'
   /\ (forall (#tt:Type) (bb:buffer tt). (frameOf bb = rid /\ live h bb /\ disjoint b bb /\ disjoint b' bb /\ disjoint b'' bb)
        ==> equal h bb h' bb)
+
+let to_set_4 (n1:nat) (n2:nat) (n3:nat) (n4:nat) :Set.set nat =
+  Set.union (Set.union (Set.union (Set.singleton n1) (Set.singleton n2)) (Set.singleton n3)) (Set.singleton n4)
 
 let modifies_buf_4 (#t:Type) (#t':Type) (#t'':Type) (#t''':Type) rid (b:buffer t) (b':buffer t') (b'':buffer t'') (b''':buffer t''') h h' =
   modifies_ref rid (to_set_4 (as_addr b) (as_addr b') (as_addr b'') (as_addr b''')) h h'
@@ -239,15 +248,15 @@ let lemma_modifies_bufs_sub rid bufs subbufs h0 h1 :
  = ()
 
 val lemma_modifies_bufs_subset: #a:Type -> #a':Type -> h0:mem -> h1:mem -> bufs:TSet.set abuffer -> b:buffer a -> b':buffer a' -> Lemma
-  (requires (~(live h0 b') /\ live h0 b /\ disjoint_from_bufs b (bufs ++ (only b')) ))
+  (requires (not_live h0 b' /\ live h0 b /\ disjoint_from_bufs b (bufs ++ (only b')) ))
   (ensures (disjoint_from_bufs b bufs))
   [SMTPatT (modifies_bufs h0.tip (bufs ++ (only b')) h0 h1); SMTPatT (live h0 b)]
 let lemma_modifies_bufs_subset #a #a' h0 h1 bufs b b' = ()
 
 val lemma_modifies_bufs_superset: #a:Type -> #a':Type -> h0:mem -> h1:mem -> bufs:TSet.set abuffer -> b:buffer a -> b':buffer a' -> Lemma
-  (requires (~(contains h0 b') /\ live h0 b /\ disjoint_from_bufs b bufs))
+  (requires (does_not_contain h0 b' /\ live h0 b /\ disjoint_from_bufs b bufs))
   (ensures (disjoint_from_bufs b (bufs ++ (only b'))))
-  [SMTPatT (modifies_bufs h0.tip bufs h0 h1); SMTPatT (~(live h0 b')); SMTPatT (live h0 b)]
+  [SMTPatT (modifies_bufs h0.tip bufs h0 h1); SMTPatT (not_live h0 b'); SMTPatT (live h0 b)]
 let lemma_modifies_bufs_superset #a #a' h0 h1 bufs b b' = ()
 
 (* Specialized lemmas *)
@@ -636,7 +645,7 @@ let lemma_modifies_0_1 (#a:Type) (b:buffer a) h0 h1 h2 : Lemma
   = ()
 
 let lemma_modifies_0_1' (#a:Type) (b:buffer a) h0 h1 h2 : Lemma
-  (requires (~(contains h0 b) /\ modifies_0 h0 h1 /\ live h1 b /\ modifies_1 b h1 h2))
+  (requires (does_not_contain h0 b /\ modifies_0 h0 h1 /\ live h1 b /\ modifies_1 b h1 h2))
   (ensures  (modifies_0 h0 h2))
   [SMTPatT (modifies_0 h0 h1); SMTPatT (modifies_1 b h1 h2)]
   = ()
@@ -651,28 +660,28 @@ let lemma_modifies_1_1 (#a:Type) (#a':Type) (b:buffer a) (b':buffer a') h0 h1 h2
   = ()
 
 let lemma_modifies_0_2 (#t:Type) (#t':Type) (b:buffer t) (b':buffer t') h0 h1 h2 : Lemma
-  (requires (live h0 b /\ ~(contains h0 b') /\ modifies_0 h0 h1 /\ live h1 b'
+  (requires (live h0 b /\ does_not_contain h0 b' /\ modifies_0 h0 h1 /\ live h1 b'
     /\ frameOf b' = h0.tip /\ modifies_2 b b' h1 h2))
   (ensures  (modifies_2_1 b h0 h2))
   [SMTPatT (modifies_2 b b' h1 h2); SMTPatT (modifies_0 h0 h1)]
   = ()
 
 let lemma_modifies_0_2' (#t:Type) (#t':Type) (b:buffer t) (b':buffer t') h0 h1 h2 : Lemma
-  (requires (live h0 b /\ ~(contains h0 b') /\ modifies_0 h0 h1 /\ live h1 b'
+  (requires (live h0 b /\ does_not_contain h0 b' /\ modifies_0 h0 h1 /\ live h1 b'
     /\ frameOf b' = h0.tip /\ modifies_2 b' b h1 h2))
   (ensures  (modifies_2_1 b h0 h2))
   [SMTPatT (modifies_2 b' b h1 h2); SMTPatT (modifies_0 h0 h1)]
   = ()
 
 let lemma_modifies_1_2 (#t:Type) (#t':Type) (b:buffer t) (b':buffer t') h0 h1 h2 : Lemma
-  (requires (live h0 b /\ modifies_1 b h0 h1 /\ ~(contains h0 b') /\ live h1 b' /\
+  (requires (live h0 b /\ modifies_1 b h0 h1 /\ does_not_contain h0 b' /\ live h1 b' /\
     modifies_2 b b' h1 h2 /\ frameOf b' = h0.tip))
   (ensures  (modifies_2_1 b h0 h2))
   [SMTPatT (modifies_1 b h0 h1); SMTPatT (modifies_2 b b' h1 h2)]
   = ()
 
 let lemma_modifies_1_2' (#t:Type) (#t':Type) (b:buffer t) (b':buffer t') h0 h1 h2 : Lemma
-  (requires (live h0 b /\ modifies_1 b h0 h1 /\ ~(contains h0 b') /\ live h1 b' /\
+  (requires (live h0 b /\ modifies_1 b h0 h1 /\ does_not_contain h0 b' /\ live h1 b' /\
     modifies_2 b' b h1 h2 /\ frameOf b' = h0.tip))
   (ensures  (modifies_2_1 b h0 h2))
   [SMTPatT (modifies_1 b h0 h1); SMTPatT (modifies_2 b' b h1 h2)]
@@ -691,7 +700,7 @@ let lemma_modifies_1_2''' (#t:Type) (#t':Type) (b:buffer t) (b':buffer t') h0 h1
   = ()
 
 let lemma_modifies_1_1_prime (#t:Type) (#t':Type) (b:buffer t) (b':buffer t') h0 h1 h2 : Lemma
-  (requires (live h0 b /\ modifies_1 b h0 h1 /\ ~(contains h0 b') /\ live h1 b' /\
+  (requires (live h0 b /\ modifies_1 b h0 h1 /\ does_not_contain h0 b' /\ live h1 b' /\
     modifies_1 b' h1 h2 /\ frameOf b' = h0.tip))
   (ensures  (modifies_2_1 b h0 h2))
   [SMTPatT (modifies_1 b h0 h1); SMTPatT (modifies_1 b' h1 h2)]
@@ -724,7 +733,7 @@ let lemma_modifies_2_1'' (#a:Type) (#a':Type) (b:buffer a) (b':buffer a') h0 h1 
 (** Concrete getters and setters *)
 val create: #a:Type -> init:a -> len:UInt32.t -> StackInline (buffer a)
   (requires (fun h -> True))
-  (ensures (fun (h0:mem) b h1 -> ~(contains h0 b)
+  (ensures (fun (h0:mem) b h1 -> does_not_contain h0 b
      /\ live h1 b /\ idx b = 0 /\ length b = v len
      /\ frameOf b = h0.tip
      /\ Map.domain h1.h == Map.domain h0.h
@@ -754,7 +763,7 @@ val createL: #a:Type0 -> init:list a -> StackInline (buffer a)
   (ensures (fun (h0:mem) b h1 ->
      let len = L.length init in
      len > 0
-     /\ ~(contains h0 b)
+     /\ does_not_contain h0 b
      /\ live h1 b /\ idx b = 0 /\ length b = len
      /\ frameOf b = h0.tip
      /\ Map.domain h1.h == Map.domain h0.h
@@ -784,14 +793,14 @@ let lemma_upd (#a:Type) (h:mem) (x:reference a{live_region h x.id}) (v:a) : Lemm
 
 val rcreate: #a:Type -> r:HH.rid -> init:a -> len:UInt32.t -> ST (buffer a)
   (requires (fun h -> is_eternal_region r))
-  (ensures (fun (h0:mem) b h1 -> ~(contains h0 b)
+  (ensures (fun (h0:mem) b h1 -> does_not_contain h0 b
     /\ live h1 b /\ idx b = 0 /\ length b = v len
     /\ Map.domain h1.h == Map.domain h0.h
     /\ h1.tip = h0.tip
     /\ modifies (Set.singleton r) h0 h1
-    /\ modifies_ref r TSet.empty h0 h1
+    /\ modifies_ref r Set.empty h0 h1
     /\ as_seq h1 b == Seq.create (v len) init
-    /\ ~(b.content.mm)))
+    /\ ~(is_mm b.content)))
 let rcreate #a r init len =
   let h0 = HST.get() in
   let s = Seq.create (v len) init in
@@ -848,13 +857,44 @@ let index #a b n =
 
 (** REMARK: the proof of this lemma relies crucially on the `a == a'` condition
     in B`uffer.disjoint`, and on the pattern in `Seq.slice_upd` *)
+private let lemma_aux_0
+  (#a:Type) (b:buffer a) (n:UInt32.t{v n < length b}) (z:a) (h0:mem) (tt:Type) (bb:buffer tt)
+  :Lemma (requires (live h0 b /\ live h0 bb /\ disjoint b bb))
+         (ensures  (live h0 b /\ live h0 bb /\
+	            (let h1 = HS.upd h0 b.content (Seq.upd (sel h0 b) (idx b + v n) z) in
+		     as_seq h0 bb == as_seq h1 bb)))
+  = if FStar.StrongExcludedMiddle.strong_excluded_middle (a == tt) &&
+      as_addr b = as_addr bb && frameOf b = frameOf bb then begin
+      Heap.sel_same_addr (Map.sel h0.h (frameOf bb)) (as_ref b) (as_ref bb)
+    end
+
+private let lemma_aux_1
+  (#a:Type) (b:buffer a) (n:UInt32.t{v n < length b}) (z:a) (h0:mem) (tt:Type)
+  :Lemma (requires (live h0 b))
+         (ensures  (live h0 b /\
+	            (forall (bb:buffer tt). (live h0 bb /\ disjoint b bb) ==>
+		                       (let h1 = HS.upd h0 b.content (Seq.upd (sel h0 b) (idx b + v n) z) in
+		                        as_seq h0 bb == as_seq h1 bb))))
+  = let open FStar.Classical in
+    forall_intro (move_requires (lemma_aux_0 b n z h0 tt))
+
+private let lemma_aux_2
+  (#a:Type) (b:buffer a) (n:UInt32.t{v n < length b}) (z:a) (h0:mem)
+  :Lemma (requires (live h0 b))
+         (ensures  (live h0 b /\
+	            (forall (tt:Type) (bb:buffer tt). (live h0 bb /\ disjoint b bb) ==>
+		                                 (let h1 = HS.upd h0 b.content (Seq.upd (sel h0 b) (idx b + v n) z) in
+		                                  as_seq h0 bb == as_seq h1 bb))))
+  = let open FStar.Classical in
+    forall_intro (move_requires (lemma_aux_1 b n z h0))
+
 private val lemma_aux: #a:Type -> b:buffer a -> n:UInt32.t{v n < length b} -> z:a
   -> h0:mem -> Lemma
   (requires (live h0 b))
   (ensures (live h0 b
     /\ modifies_1 b h0 (HS.upd h0 b.content (Seq.upd (sel h0 b) (idx b + v n) z)) ))
   [SMTPat (HS.upd h0 b.content (Seq.upd (sel h0 b) (idx b + v n) z))]
-let lemma_aux #a b n z h0 = ()
+let lemma_aux #a b n z h0 = lemma_aux_2 b n z h0
 
 val upd: #a:Type -> b:buffer a -> n:UInt32.t -> z:a -> Stack unit
   (requires (fun h -> live h b /\ v n < length b))
@@ -862,9 +902,11 @@ val upd: #a:Type -> b:buffer a -> n:UInt32.t -> z:a -> Stack unit
     /\ modifies_1 b h0 h1
     /\ as_seq h1 b == Seq.upd (as_seq h0 b) (v n) z ))
 let upd #a b n z =
+  let h0 = HST.get () in
   let s0 = !b.content in
   let s = Seq.upd s0 (v b.idx + v n) z in
   b.content := s;
+  lemma_aux b n z h0;
   let h = HST.get() in
   Seq.lemma_eq_intro (as_seq h b) (Seq.slice s (idx b) (idx b + length b));
   Seq.upd_slice s0 (idx b) (idx b + length b) (v n) z
@@ -1089,7 +1131,7 @@ let modifies_subbuffer_2 (#t:Type) (#t':Type) h0 h1 (sub:buffer t) (a':buffer t'
   (ensures  (modifies_2 a a' h0 h1 /\ modifies_2 a' a h0 h1 /\ live h1 a))
   [SMTPatT (modifies_2 sub a' h0 h1); SMTPatT (includes a sub)]
   = ()
-
+    
 let modifies_subbuffer_2' (#t:Type) (#t':Type) h0 h1 (sub:buffer t) (a':buffer t') (a:buffer t) : Lemma
   (requires (live h0 a /\ live h0 a' /\ includes a sub /\ modifies_2 a' sub h0 h1 ))
   (ensures  (modifies_2 a a' h0 h1 /\ live h1 a))
